Batteries/Data/Iterators/Lemmas/Scan.lean
@@ -9,34 +9,31 @@ public import Batteries.Data.Iterators.Scan
 public import Batteries.Data.List.Scan
 public import Batteries.Data.Array.Scan
 
-namespace Std.Iterators
+namespace Std
+open Std.Iterators Std.Iterators.Types
 
-theorem toIterM_eq_mk {state : ScanM α m n β γ f} :
-    (toIterM state n γ : IterM n γ) = { internalState := state } := rfl
+theorem IterM.mk_def {state : ScanM α m n β γ f} :
+    (IterM.mk state n γ : IterM n γ) = { internalState := state } := rfl
 
 theorem toList_scanM_emittedTrue [Iterator α Id β] [Finite α Id] [Monad m] [LawfulMonad m]
-  [IteratorCollect α Id Id (β := β)] [LawfulIteratorCollect α Id Id (β := β)]
   {f : γ → β → m γ} {acc : γ} {it : IterM (α := α) Id β} :
-    (toIterM (m := m) (β := γ) (⟨it.internalState, acc, true⟩ : ScanM α Id m β γ f)).toList
+    (IterM.mk (m := m) (β := γ) (ScanM.mk (m := Id) (f := f) it.internalState acc true)).toList
       = (return (← List.scanlM f acc (← it.toList)).tail) := by
   induction it using IterM.inductSteps generalizing acc
   rename_i it ihy ihs
   rw [IterM.toList_eq_match_step, IterM.toList_eq_match_step]
-  simp only [IterM.step, liftM_bind, ScanM.instIterator, internalState_toIterM]
-  simp only [Bool.true_eq_false, ↓reduceDIte, bind_assoc]
-  apply bind_congr
-  intro step
-  match hstep : step.inflate with
+  simp only [Iterator.step, liftM, monadLift, Id.run, bind_pure_comp, pure_bind,
+    IterM.mk_def, IterM.step, Bool.true_eq_false, ↓reduceDIte, bind, pure] at ⊢ ihy ihs
+  match hstep : it.step.inflate with
   | ⟨.yield inner' out, hp⟩ =>
-    simp only [liftM, monadLift, Id.run, pure_bind, toIterM] at ⊢ ihy
-    simp only [bind_pure_comp, bind_map_left, Shrink.inflate_deflate,
-      List.scanlM_cons, map_bind, Functor.map]
+    simp only [bind_map_left, Shrink.inflate_deflate, List.scanlM_cons, bind_pure_comp, map_bind]
+    skip
     apply bind_congr
     intro a
     rw [ihy hp, ← List.scanlM_cons_head_tail]
     simp
   | ⟨.skip inner', hp⟩ =>
-    simp_all [liftM, monadLift, Id.run, toIterM]
+    simp_all
   | ⟨.done, hp⟩ =>
     simp_all
 
@@ -44,18 +41,16 @@ public section
 
 @[simp]
 theorem IterM.toList_scanM [Iterator α Id β] [Finite α Id] [Monad m] [LawfulMonad m]
-    [IteratorCollect α Id Id (β := β)] [LawfulIteratorCollect α Id Id (β := β)]
     {f : γ → β → m γ} {init : γ} (it : IterM (α := α) Id β) :
     (it.scanM f init).toList = List.scanlM f init it.toList := by
   simp only [IterM.scanM]
   rw [IterM.toList_eq_match_step]
-  simp only [Iterator.step, ScanM.instIterator, IterM.step]
+  simp only [Iterator.step, IterM.step, ← mk_def, bind_pure_comp]
   have := List.scanlM_cons_head_tail (as := it.toList) (init := init) (f := f)
-  simp_all [← toIterM_eq_mk, liftM, monadLift, Id.run, toList_scanM_emittedTrue]
+  simp_all [liftM, monadLift, Id.run, toList_scanM_emittedTrue]
 
 @[simp]
 theorem Iter.toList_scanM [Iterator α Id β] [Finite α Id] [Monad m] [LawfulMonad m]
-    [IteratorCollect α Id Id (β := β)] [LawfulIteratorCollect α Id Id (β := β)]
     {f : γ → β → m γ} {init : γ} (it : Iter (α := α) β) :
     (it.scanM f init).toList = List.scanlM f init it.toList := by
   unfold Iter.scanM
@@ -63,21 +58,18 @@ theorem Iter.toList_scanM [Iterator α Id β] [Finite α Id] [Monad m] [LawfulMo
 
 @[simp]
 theorem IterM.toList_scan [Iterator α Id β] [Finite α Id]
-    [IteratorCollect α Id Id (β := β)] [LawfulIteratorCollect α Id Id (β := β)]
     {f : γ → β → γ} {init : γ} (it : IterM (α := α) Id β) :
     (it.scan f init).toList = List.scanl f init it.toList := by
   simp [List.scanl, scan, pure, Id.run]
 
 @[simp]
 theorem Iter.toList_scan [Iterator α Id β] [Finite α Id]
-    [IteratorCollect α Id Id (β := β)] [LawfulIteratorCollect α Id Id (β := β)]
     {f : γ → β → γ} {init : γ} (it : Iter (α := α) β) :
     (it.scan f init).toList = List.scanl f init it.toList := by
   simp [Iter.scan, List.scanl]
 
 @[simp]
 theorem IterM.toArray_scanM [Iterator α Id β] [Finite α Id] [Monad m] [LawfulMonad m]
-    [IteratorCollect α Id Id (β := β)] [LawfulIteratorCollect α Id Id (β := β)]
     {f : γ → β → m γ} {init : γ} (it : IterM (α := α) Id β) :
     (it.scanM f init).toArray = Array.scanlM f init it.toArray := by
   repeat rw [← toArray_toList]
@@ -86,7 +78,6 @@ theorem IterM.toArray_scanM [Iterator α Id β] [Finite α Id] [Monad m] [Lawful
 
 @[simp]
 theorem Iter.toArray_scanM [Iterator α Id β] [Finite α Id] [Monad m] [LawfulMonad m]
-    [IteratorCollect α Id Id (β := β)] [LawfulIteratorCollect α Id Id (β := β)]
     {f : γ → β → m γ} {init : γ} (it : Iter (α := α) β) :
     (it.scanM f init).toArray = Array.scanlM f init it.toArray := by
   unfold Iter.scanM
@@ -94,18 +85,16 @@ theorem Iter.toArray_scanM [Iterator α Id β] [Finite α Id] [Monad m] [LawfulM
 
 @[simp]
 theorem IterM.toArray_scan [Iterator α Id β] [Finite α Id]
-    [IteratorCollect α Id Id (β := β)] [LawfulIteratorCollect α Id Id (β := β)]
     {f : γ → β → γ} {init : γ} (it : IterM (α := α) Id β) :
     (it.scan f init).toArray = Array.scanl f init it.toArray := by
   simp [Array.scanl_eq_scanlM, scan, pure, Id.run]
 
 @[simp]
 theorem Iter.toArray_scan [Iterator α Id β] [Finite α Id]
-    [IteratorCollect α Id Id (β := β)] [LawfulIteratorCollect α Id Id (β := β)]
     {f : γ → β → γ} {init : γ} (it : Iter (α := α) β) :
     (it.scan f init).toArray = Array.scanl f init it.toArray := by
   unfold scan
   apply IterM.toArray_scan
 
 end
-end Std.Iterators
+end Std
